@prefix : <https://onerecord.iata.org/ns/glecf#> .
@prefix dc: <http://purl.org/dc/elements/1.1/> .
@prefix owl: <http://www.w3.org/2002/07/owl#> .
@prefix rdf: <http://www.w3.org/1999/02/22-rdf-syntax-ns#> .
@prefix xml: <http://www.w3.org/XML/1998/namespace> .
@prefix xsd: <http://www.w3.org/2001/XMLSchema#> .
@prefix rdfs: <http://www.w3.org/2000/01/rdf-schema#> .
@prefix cargo: <https://onerecord.iata.org/ns/cargo#> .
@prefix terms: <http://purl.org/dc/terms/> .
@base <https://onerecord.iata.org/ns/glecf> .

<https://onerecord.iata.org/ns/glecf> rdf:type owl:Ontology ;
                                       owl:versionIRI <https://onerecord.iata.org/ns/glecf/0.1.1> ;
                                       dc:description """Extension to the ONE Record vocabulary integrating the GLEC framework, described using W3C RDF Schema and the Web Ontology Language.

Depends on the ONE Record data model (cargo ontology) of version 3.0.0 RC 4.1 or later:
https://github.com/IATA-Cargo/ONE-Record/blob/master/working_draft/ontology/IATA-1R-DM-Ontology.ttl

For further information on the GLEC framework, please refer to the Smart Freight Centre and their provided sources:
https://www.smartfreightcentre.org/en/
https://www.feport.eu/images/downloads/glec-framework-20.pdf"""@en ;
                                       dc:title "ONE Record GLEC framework Integration Ontology"@en ;
                                       terms:abstract "The ontology of the ONE Record standard is the core data model underlying the Linked Data solution drafted by the ONE Record standard: https://github.com/IATA-Cargo/ONE-Record. ONE Record is a standard for data sharing and creates a single record view of the shipment. This standard defines a common data model for the data that is shared via standardized and secured web API."@en ;
                                       terms:modified "19-06-2023" ;
                                       rdfs:comment """Details availalble on GitHub https://github.com/DrPhilippBillion/Co2-Transparency-in-ONE-Record_for_2023_Hackathon

0.1.1
- Initial trial version for the 2023 Seeheim ONE Record Hackathon"""@en ;
                                       rdfs:isDefinedBy "https://www.iata.org/one-record/ns/glecf"@en ;
                                       rdfs:label "ONE Record GLEC framework Integration Ontology"@en ;
                                       owl:versionInfo "0.1.1"@en .

#################################################################
#    Annotation properties
#################################################################

###  http://purl.org/dc/elements/1.1/description
dc:description rdf:type owl:AnnotationProperty .


###  http://purl.org/dc/elements/1.1/title
dc:title rdf:type owl:AnnotationProperty .


###  http://purl.org/dc/terms/abstract
terms:abstract rdf:type owl:AnnotationProperty .


###  http://purl.org/dc/terms/modified
terms:modified rdf:type owl:AnnotationProperty .


###  http://purl.org/dc/terms/title
terms:title rdf:type owl:AnnotationProperty .


###  http://www.w3.org/2002/07/owl#comment
owl:comment rdf:type owl:AnnotationProperty .


###  http://www.w3.org/2002/07/owl#maxCardinality
owl:maxCardinality rdf:type owl:AnnotationProperty .


###  http://www.w3.org/2002/07/owl#minCardinality
owl:minCardinality rdf:type owl:AnnotationProperty .


#################################################################
#    Datatypes
#################################################################

###  http://www.w3.org/2001/XMLSchema#date
xsd:date rdf:type rdfs:Datatype .


###  http://www.w3.org/2001/XMLSchema#duration
xsd:duration rdf:type rdfs:Datatype .


###  http://www.w3.org/2002/07/owl#thing
owl:thing rdf:type rdfs:Datatype .


#################################################################
#    Object Properties
#################################################################

###  https://onerecord.iata.org/ns/glecf#dataQualityIndex
:dataQualityIndex rdf:type owl:ObjectProperty ;
                  rdfs:domain :ClimateEffect ;
                  rdfs:range :QualityLevel ;
                  rdfs:comment "TBC (Definition from E2E. Calculated with respect to % of emissions)"@en ;
                  rdfs:label ":dataQualityIndex"@en .


###  https://onerecord.iata.org/ns/glecf#elementClimateEffects
:elementClimateEffects rdf:type owl:ObjectProperty ;
                       rdfs:domain :TransportChainElement ;
                       rdfs:range :ClimateEffect ;
                       rdfs:comment "References to all piece-specific ClimateEffects this TransportChainElement is the base of"@en ;
                       rdfs:label ":elementClimateEffects"@en .


###  https://onerecord.iata.org/ns/glecf#energyFeedstocks
:energyFeedstocks rdf:type owl:ObjectProperty ;
                  rdfs:domain cargo:TransportMovement ;
                  rdfs:range :EnergyFeedstock ;
                  rdfs:comment "Information about the feedstocks used to produce the energyCarrier"@en ;
                  rdfs:label ":energyFeedstocks"@en .


###  https://onerecord.iata.org/ns/glecf#energyMeasured
:energyMeasured rdf:type owl:ObjectProperty ;
                rdfs:domain cargo:TransportMovement ;
                rdfs:range cargo:Value ;
                rdfs:comment "Energy measured for this TransportMovement (measured in l, kg, kWh or MJ per km)"@en ;
                rdfs:label ":energyMeasured"@en .


###  https://onerecord.iata.org/ns/glecf#ofPiece
:ofPiece rdf:type owl:ObjectProperty ;
         rdfs:domain :ClimateEffect ;
         rdfs:range cargo:Piece ;
         rdfs:comment "Reference to the TransportChainElement this ClimateEffect results from"@en ;
         rdfs:label ":ofPiece"@en .


###  https://onerecord.iata.org/ns/glecf#ofTransportChainElement
:ofTransportChainElement rdf:type owl:ObjectProperty ;
                         rdfs:domain :ClimateEffect ;
                         rdfs:range :TransportChainElement ;
                         rdfs:comment "Reference to the Piece this ClimateEffect describes"@en ;
                         rdfs:label ":ofTransportChainElement"@en .


###  https://onerecord.iata.org/ns/glecf#pieceClimateEffect
:pieceClimateEffect rdf:type owl:ObjectProperty ;
                    rdfs:domain cargo:Piece ;
                    rdfs:range :ClimateEffect ;
                    rdfs:comment "References to all ClimateEffects this Piece produced in its lifecycle"@en ;
                    rdfs:label ":pieceClimateEffect"@en .


###  https://onerecord.iata.org/ns/glecf#tankToWheelCH4
:tankToWheelCH4 rdf:type owl:ObjectProperty ;
                rdfs:domain :TransportChainElement ;
                rdfs:range cargo:Value ;
                rdfs:comment "Methane released to atmosphere as a result of vehicle operation (measured in kg)"@en ;
                rdfs:label ":tankToWheelCH4"@en .


###  https://onerecord.iata.org/ns/glecf#tankToWheelCO2
:tankToWheelCO2 rdf:type owl:ObjectProperty ;
                rdfs:domain :TransportChainElement ;
                rdfs:range cargo:Value ;
                rdfs:comment "CO2 released to atmosphere as a result of vehicle operation (measured in kg)"@en ;
                rdfs:label ":tankToWheelCO2"@en .


###  https://onerecord.iata.org/ns/glecf#tankToWheelCO2equivalent
:tankToWheelCO2equivalent rdf:type owl:ObjectProperty ;
                          rdfs:domain :ClimateEffect ;
                          rdfs:range cargo:Value ;
                          rdfs:comment "Greenhouse gases released to atmosphere as a result of vehicle operation (measured in kg)"@en ;
                          rdfs:label ":tankToWheelCO2equivalent"@en .


###  https://onerecord.iata.org/ns/glecf#tankToWheelNOX
:tankToWheelNOX rdf:type owl:ObjectProperty ;
                rdfs:domain :TransportChainElement ;
                rdfs:range cargo:Value ;
                rdfs:comment "Nitrogen oxide released to atmosphere as a result of vehicle operation (measured in kg)"@en ;
                rdfs:label ":tankToWheelNOX"@en .


###  https://onerecord.iata.org/ns/glecf#tankToWheelPM
:tankToWheelPM rdf:type owl:ObjectProperty ;
               rdfs:domain :TransportChainElement ;
               rdfs:range cargo:Value ;
               rdfs:comment "Particulate matter (PM10 and PM2.5) released to atmosphere as a result of vehicle operation (measured in kg)"@en ;
               rdfs:label ":tankToWheelPM"@en .


###  https://onerecord.iata.org/ns/glecf#tankToWheelSOX
:tankToWheelSOX rdf:type owl:ObjectProperty ;
                rdfs:domain :TransportChainElement ;
                rdfs:range cargo:Value ;
                rdfs:comment "Sulphur oxide released to atmosphere as a result of vehicle operation (measured in kg)"@en ;
                rdfs:label ":tankToWheelSOX"@en .


###  https://onerecord.iata.org/ns/glecf#transportChainElements
:transportChainElements rdf:type owl:ObjectProperty ;
                        rdfs:domain cargo:TransportMovement ;
                        rdfs:range :TransportChainElement ;
                        rdfs:comment "References to all TransportChainElements this TransportMovement describes"@en ;
                        rdfs:label ":transportChainElements"@en .


###  https://onerecord.iata.org/ns/glecf#wellToWheelCO2
:wellToWheelCO2 rdf:type owl:ObjectProperty ;
                rdfs:domain :TransportChainElement ;
                rdfs:range cargo:Value ;
                rdfs:comment "CO2 released to atmosphere during the process of producing, storing, processing and distributing an energy carrier for vehicle operation + CO2 released to atmosphere as a result of vehicle operation (measured in kg)"@en ;
                rdfs:label ":wellToWheelCO2"@en .


###  https://onerecord.iata.org/ns/glecf#wellToWheelCO2equivalent
:wellToWheelCO2equivalent rdf:type owl:ObjectProperty ;
                          rdfs:domain :ClimateEffect ;
                          rdfs:range cargo:Value ;
                          rdfs:comment "Greenhouse gases released to atmosphere during the process of producing, storing, processing and distributing an energy carrier for vehicle operation + Greenhouse gases released to atmosphere as a result of vehicle operation (measured in kg)"@en ;
                          rdfs:label ":wellToWheelCO2equivalent"@en .


###  https://onerecord.iata.org/ns/glecf#wellToWheelEmissionIntensity
:wellToWheelEmissionIntensity rdf:type owl:ObjectProperty ;
                              rdfs:domain :TransportChainElement ;
                              rdfs:range cargo:Value ;
                              rdfs:comment "Coefficient relating specified transport activity with GHG emissions"@en ;
                              rdfs:label ":wellToWheelEmissionIntensity"@en .


#################################################################
#    Data properties
#################################################################

###  https://onerecord.iata.org/ns/glecf#accreditation
:accreditation rdf:type owl:DatatypeProperty ;
               rdfs:domain owl:Thing ;
               rdfs:range xsd:boolean ;
               rdfs:comment "Statement of accreditation of the calculation methodology"@en ;
               rdfs:label ":accreditation"@en .


###  https://onerecord.iata.org/ns/glecf#emissionClass
:emissionClass rdf:type owl:DatatypeProperty ;
               rdfs:domain cargo:TransportMeans ;
               rdfs:range xsd:string ;
               rdfs:comment "Identification of the vehicle emission class (Road). Depending on the geography of operations, this can be adapted"@en ;
               rdfs:label ":emissionClass"@en .


###  https://onerecord.iata.org/ns/glecf#energyCarrier
:energyCarrier rdf:type owl:DatatypeProperty ;
               rdfs:domain cargo:TransportMovement ;
               rdfs:range xsd:string ;
               rdfs:comment "Energy carrier used for powering this TransportMovement, such as Diesel, HVO, petrol, CNG, LNG, LPG, HFO, MGO, Aviation fuel, Hydrogen, Methanol, Electric, etc."@en ;
               rdfs:label ":energyCarrier"@en .


###  https://onerecord.iata.org/ns/glecf#energyRemarks
:energyRemarks rdf:type owl:DatatypeProperty ;
               rdfs:domain cargo:TransportMovement ;
               rdfs:range xsd:string ;
               rdfs:comment "Description of the measuredEnergy and energyCarrier"@en ;
               rdfs:label ":energyRemarks"@en .


###  https://onerecord.iata.org/ns/glecf#feedstock
:feedstock rdf:type owl:DatatypeProperty ;
           rdfs:domain :EnergyFeedstock ;
           rdfs:range xsd:string ;
           rdfs:comment "Feedstock (e.g. fossil, natural gas, grid, renewable electricity, waste)"@en ;
           rdfs:label ":feedstock"@en .


###  https://onerecord.iata.org/ns/glecf#feedstockShare
:feedstockShare rdf:type owl:DatatypeProperty ;
                rdfs:domain :EnergyFeedstock ;
                rdfs:range xsd:double ;
                rdfs:comment "Share of the feedstock of the energy carrier (0 in case only 1 feedstock is applicable, e.g. 0.05 to cover a 5% blend)"@en ;
                rdfs:label ":feedstockShare"@en .


###  https://onerecord.iata.org/ns/glecf#loadFactor
:loadFactor rdf:type owl:DatatypeProperty ;
            rdfs:domain cargo:TransportMovement ;
            rdfs:range xsd:double ;
            rdfs:comment "Ratio of the mass of the actual load to the maximum legally authorized load of a particular vehicle on a TOC level"@en ;
            rdfs:label ":loadFactor"@en .


###  https://onerecord.iata.org/ns/glecf#loadFactorRemarks
:loadFactorRemarks rdf:type owl:DatatypeProperty ;
                   rdfs:domain cargo:TransportMovement ;
                   rdfs:range xsd:string ;
                   rdfs:comment "Description of derivation of the load factor"@en ;
                   rdfs:label ":loadFactorRemarks"@en .


###  https://onerecord.iata.org/ns/glecf#methodLink
:methodLink rdf:type owl:DatatypeProperty ;
            rdfs:domain :ClimateEffect ;
            rdfs:range xsd:string ;
            rdfs:comment "Link referring to documentation of the CO2 equivalent calculation method"@en ;
            rdfs:label ":methodLink"@en .


###  https://onerecord.iata.org/ns/glecf#methodName
:methodName rdf:type owl:DatatypeProperty ;
            rdfs:domain :ClimateEffect ;
            rdfs:range xsd:string ;
            rdfs:comment "Name of the CO2 equivalent calculation method"@en ;
            rdfs:label ":methodName"@en .


###  https://onerecord.iata.org/ns/glecf#methodVersion
:methodVersion rdf:type owl:DatatypeProperty ;
               rdfs:domain :ClimateEffect ;
               rdfs:range xsd:string ;
               rdfs:comment "Version of the CO2 equivalent calculation method"@en ;
               rdfs:label ":methodVersion"@en .


###  https://onerecord.iata.org/ns/glecf#positioningMovement
:positioningMovement rdf:type owl:DatatypeProperty ;
                     rdfs:domain cargo:TransportMovement ;
                     rdfs:range xsd:boolean ;
                     rdfs:comment "Indicator whether the TransportMovement serves repositioning"@en ;
                     rdfs:label ":positioningMovement"@en .


###  https://onerecord.iata.org/ns/glecf#verification
:verification rdf:type owl:DatatypeProperty ;
              rdfs:domain owl:Thing ;
              rdfs:range xsd:boolean ;
              rdfs:comment "Statement of external verification of the input data"@en ;
              rdfs:label ":verification"@en .


###  https://onerecord.iata.org/ns/glecf#wellToWheelFuelEmissionFactor
:wellToWheelFuelEmissionFactor rdf:type owl:DatatypeProperty ;
                               rdfs:domain :TransportChainElement ;
                               rdfs:range xsd:double ;
                               rdfs:comment """Well to wheel fuel emission factor (certified) (measured in kg CO2e per 
kg, l, kWh or MJ)"""@en ;
                               rdfs:label ":wellToWheelFuelEmissionFactor"@en .


#################################################################
#    Classes
#################################################################

###  https://onerecord.iata.org/ns/cargo#LogisticsObject
cargo:LogisticsObject rdf:type owl:Class .


###  https://onerecord.iata.org/ns/cargo#Piece
cargo:Piece rdf:type owl:Class ;
            rdfs:subClassOf [ rdf:type owl:Restriction ;
                              owl:onProperty :pieceClimateEffect ;
                              owl:allValuesFrom :ClimateEffect
                            ] .


###  https://onerecord.iata.org/ns/cargo#TransportMeans
cargo:TransportMeans rdf:type owl:Class ;
                     rdfs:subClassOf [ rdf:type owl:Restriction ;
                                       owl:onProperty :emissionClass ;
                                       owl:allValuesFrom xsd:string
                                     ] ,
                                     [ rdf:type owl:Restriction ;
                                       owl:onProperty :emissionClass ;
                                       owl:maxCardinality "1"^^xsd:nonNegativeInteger
                                     ] .


###  https://onerecord.iata.org/ns/cargo#TransportMovement
cargo:TransportMovement rdf:type owl:Class ;
                        rdfs:subClassOf [ rdf:type owl:Restriction ;
                                          owl:onProperty :energyFeedstocks ;
                                          owl:allValuesFrom :EnergyFeedstock
                                        ] ,
                                        [ rdf:type owl:Restriction ;
                                          owl:onProperty :energyMeasured ;
                                          owl:allValuesFrom cargo:Value
                                        ] ,
                                        [ rdf:type owl:Restriction ;
                                          owl:onProperty :transportChainElements ;
                                          owl:allValuesFrom :TransportChainElement
                                        ] ,
                                        [ rdf:type owl:Restriction ;
                                          owl:onProperty :energyMeasured ;
                                          owl:maxCardinality "1"^^xsd:nonNegativeInteger
                                        ] ,
                                        [ rdf:type owl:Restriction ;
                                          owl:onProperty :energyCarrier ;
                                          owl:allValuesFrom xsd:string
                                        ] ,
                                        [ rdf:type owl:Restriction ;
                                          owl:onProperty :energyRemarks ;
                                          owl:allValuesFrom xsd:string
                                        ] ,
                                        [ rdf:type owl:Restriction ;
                                          owl:onProperty :loadFactor ;
                                          owl:allValuesFrom xsd:double
                                        ] ,
                                        [ rdf:type owl:Restriction ;
                                          owl:onProperty :loadFactorRemarks ;
                                          owl:allValuesFrom xsd:string
                                        ] ,
                                        [ rdf:type owl:Restriction ;
                                          owl:onProperty :positioningMovement ;
                                          owl:allValuesFrom xsd:boolean
                                        ] ,
                                        [ rdf:type owl:Restriction ;
                                          owl:onProperty :energyCarrier ;
                                          owl:maxCardinality "1"^^xsd:nonNegativeInteger
                                        ] ,
                                        [ rdf:type owl:Restriction ;
                                          owl:onProperty :energyRemarks ;
                                          owl:maxCardinality "1"^^xsd:nonNegativeInteger
                                        ] ,
                                        [ rdf:type owl:Restriction ;
                                          owl:onProperty :loadFactor ;
                                          owl:maxCardinality "1"^^xsd:nonNegativeInteger
                                        ] ,
                                        [ rdf:type owl:Restriction ;
                                          owl:onProperty :loadFactorRemarks ;
                                          owl:maxCardinality "1"^^xsd:nonNegativeInteger
                                        ] ,
                                        [ rdf:type owl:Restriction ;
                                          owl:onProperty :positioningMovement ;
                                          owl:maxCardinality "1"^^xsd:nonNegativeInteger
                                        ] .


###  https://onerecord.iata.org/ns/cargo#Value
cargo:Value rdf:type owl:Class .


###  https://onerecord.iata.org/ns/glecf#ClimateEffect
:ClimateEffect rdf:type owl:Class ;
               rdfs:subClassOf cargo:LogisticsObject ,
                               [ rdf:type owl:Restriction ;
                                 owl:onProperty :dataQualityIndex ;
                                 owl:allValuesFrom :QualityLevel
                               ] ,
                               [ rdf:type owl:Restriction ;
                                 owl:onProperty :ofPiece ;
                                 owl:allValuesFrom cargo:Piece
                               ] ,
                               [ rdf:type owl:Restriction ;
                                 owl:onProperty :ofTransportChainElement ;
                                 owl:allValuesFrom :TransportChainElement
                               ] ,
                               [ rdf:type owl:Restriction ;
                                 owl:onProperty :tankToWheelCO2equivalent ;
                                 owl:allValuesFrom cargo:Value
                               ] ,
                               [ rdf:type owl:Restriction ;
                                 owl:onProperty :wellToWheelCO2equivalent ;
                                 owl:allValuesFrom cargo:Value
                               ] ,
                               [ rdf:type owl:Restriction ;
                                 owl:onProperty :dataQualityIndex ;
                                 owl:maxCardinality "1"^^xsd:nonNegativeInteger
                               ] ,
                               [ rdf:type owl:Restriction ;
                                 owl:onProperty :ofPiece ;
                                 owl:maxCardinality "1"^^xsd:nonNegativeInteger
                               ] ,
                               [ rdf:type owl:Restriction ;
                                 owl:onProperty :ofTransportChainElement ;
                                 owl:maxCardinality "1"^^xsd:nonNegativeInteger
                               ] ,
                               [ rdf:type owl:Restriction ;
                                 owl:onProperty :tankToWheelCO2equivalent ;
                                 owl:maxCardinality "1"^^xsd:nonNegativeInteger
                               ] ,
                               [ rdf:type owl:Restriction ;
                                 owl:onProperty :wellToWheelCO2equivalent ;
                                 owl:maxCardinality "1"^^xsd:nonNegativeInteger
                               ] ,
                               [ rdf:type owl:Restriction ;
                                 owl:onProperty :accreditation ;
                                 owl:allValuesFrom xsd:boolean
                               ] ,
                               [ rdf:type owl:Restriction ;
                                 owl:onProperty :methodLink ;
                                 owl:allValuesFrom xsd:string
                               ] ,
                               [ rdf:type owl:Restriction ;
                                 owl:onProperty :methodName ;
                                 owl:allValuesFrom xsd:string
                               ] ,
                               [ rdf:type owl:Restriction ;
                                 owl:onProperty :methodVersion ;
                                 owl:allValuesFrom xsd:string
                               ] ,
                               [ rdf:type owl:Restriction ;
                                 owl:onProperty :verification ;
                                 owl:allValuesFrom xsd:boolean
                               ] ,
                               [ rdf:type owl:Restriction ;
                                 owl:onProperty :accreditation ;
                                 owl:maxCardinality "1"^^xsd:nonNegativeInteger
                               ] ,
                               [ rdf:type owl:Restriction ;
                                 owl:onProperty :methodLink ;
                                 owl:maxCardinality "1"^^xsd:nonNegativeInteger
                               ] ,
                               [ rdf:type owl:Restriction ;
                                 owl:onProperty :methodName ;
                                 owl:maxCardinality "1"^^xsd:nonNegativeInteger
                               ] ,
                               [ rdf:type owl:Restriction ;
                                 owl:onProperty :methodVersion ;
                                 owl:maxCardinality "1"^^xsd:nonNegativeInteger
                               ] ,
                               [ rdf:type owl:Restriction ;
                                 owl:onProperty :verification ;
                                 owl:maxCardinality "1"^^xsd:nonNegativeInteger
                               ] ;
               rdfs:comment "A ClimateEffect holds the calculated emissions of exactly ONE piece on exactly ONE TransportMovement through a TransportChainElement (TCE).  A ClimateEffect must have a connection to one Piece and one TCE. On the other hand, a TCE can have many ClimateEffects for all Pieces covered, and a Piece can have many ClimateEffects."@en ;
               rdfs:label "ClimateEffect"@en .


###  https://onerecord.iata.org/ns/glecf#EnergyFeedstock
:EnergyFeedstock rdf:type owl:Class ;
                 rdfs:subClassOf [ rdf:type owl:Restriction ;
                                   owl:onProperty :feedstock ;
                                   owl:allValuesFrom xsd:string
                                 ] ,
                                 [ rdf:type owl:Restriction ;
                                   owl:onProperty :feedstockShare ;
                                   owl:allValuesFrom xsd:double
                                 ] ,
                                 [ rdf:type owl:Restriction ;
                                   owl:onProperty :feedstock ;
                                   owl:maxCardinality "1"^^xsd:nonNegativeInteger
                                 ] ,
                                 [ rdf:type owl:Restriction ;
                                   owl:onProperty :feedstockShare ;
                                   owl:maxCardinality "1"^^xsd:nonNegativeInteger
                                 ] ;
                 rdfs:comment "Feedstock and share of it used to create the energy carrier of a TransportMovement. Energy feedstock may be fossil, natural gas, grid, renewable electricity or waste, for example."@en ;
                 rdfs:label "EnergyFeedstock"@en .


###  https://onerecord.iata.org/ns/glecf#QualityLevel
:QualityLevel rdf:type owl:Class ;
              owl:equivalentClass [ rdf:type owl:Class ;
                                    owl:oneOf ( :LEVEL_1
                                                :LEVEL_2
                                                :LEVEL_3
                                                :LEVEL_4
                                              )
                                  ] .


###  https://onerecord.iata.org/ns/glecf#TransportChainElement
:TransportChainElement rdf:type owl:Class ;
                       rdfs:subClassOf cargo:LogisticsObject ,
                                       [ rdf:type owl:Restriction ;
                                         owl:onProperty :elementClimateEffects ;
                                         owl:allValuesFrom :ClimateEffect
                                       ] ,
                                       [ rdf:type owl:Restriction ;
                                         owl:onProperty :tankToWheelCH4 ;
                                         owl:allValuesFrom cargo:Value
                                       ] ,
                                       [ rdf:type owl:Restriction ;
                                         owl:onProperty :tankToWheelCO2 ;
                                         owl:allValuesFrom cargo:Value
                                       ] ,
                                       [ rdf:type owl:Restriction ;
                                         owl:onProperty :tankToWheelNOX ;
                                         owl:allValuesFrom cargo:Value
                                       ] ,
                                       [ rdf:type owl:Restriction ;
                                         owl:onProperty :tankToWheelPM ;
                                         owl:allValuesFrom cargo:Value
                                       ] ,
                                       [ rdf:type owl:Restriction ;
                                         owl:onProperty :tankToWheelSOX ;
                                         owl:allValuesFrom cargo:Value
                                       ] ,
                                       [ rdf:type owl:Restriction ;
                                         owl:onProperty :wellToWheelCO2 ;
                                         owl:allValuesFrom cargo:Value
                                       ] ,
                                       [ rdf:type owl:Restriction ;
                                         owl:onProperty :wellToWheelEmissionIntensity ;
                                         owl:allValuesFrom cargo:Value
                                       ] ,
                                       [ rdf:type owl:Restriction ;
                                         owl:onProperty :tankToWheelCH4 ;
                                         owl:maxCardinality "1"^^xsd:nonNegativeInteger
                                       ] ,
                                       [ rdf:type owl:Restriction ;
                                         owl:onProperty :tankToWheelCO2 ;
                                         owl:maxCardinality "1"^^xsd:nonNegativeInteger
                                       ] ,
                                       [ rdf:type owl:Restriction ;
                                         owl:onProperty :tankToWheelNOX ;
                                         owl:maxCardinality "1"^^xsd:nonNegativeInteger
                                       ] ,
                                       [ rdf:type owl:Restriction ;
                                         owl:onProperty :tankToWheelPM ;
                                         owl:maxCardinality "1"^^xsd:nonNegativeInteger
                                       ] ,
                                       [ rdf:type owl:Restriction ;
                                         owl:onProperty :tankToWheelSOX ;
                                         owl:maxCardinality "1"^^xsd:nonNegativeInteger
                                       ] ,
                                       [ rdf:type owl:Restriction ;
                                         owl:onProperty :wellToWheelCO2 ;
                                         owl:maxCardinality "1"^^xsd:nonNegativeInteger
                                       ] ,
                                       [ rdf:type owl:Restriction ;
                                         owl:onProperty :wellToWheelEmissionIntensity ;
                                         owl:maxCardinality "1"^^xsd:nonNegativeInteger
                                       ] ,
                                       [ rdf:type owl:Restriction ;
                                         owl:onProperty :accreditation ;
                                         owl:allValuesFrom xsd:boolean
                                       ] ,
                                       [ rdf:type owl:Restriction ;
                                         owl:onProperty :verification ;
                                         owl:allValuesFrom xsd:boolean
                                       ] ,
                                       [ rdf:type owl:Restriction ;
                                         owl:onProperty :wellToWheelFuelEmissionFactor ;
                                         owl:allValuesFrom xsd:double
                                       ] ,
                                       [ rdf:type owl:Restriction ;
                                         owl:onProperty :accreditation ;
                                         owl:maxCardinality "1"^^xsd:nonNegativeInteger
                                       ] ,
                                       [ rdf:type owl:Restriction ;
                                         owl:onProperty :verification ;
                                         owl:maxCardinality "1"^^xsd:nonNegativeInteger
                                       ] ,
                                       [ rdf:type owl:Restriction ;
                                         owl:onProperty :wellToWheelFuelEmissionFactor ;
                                         owl:maxCardinality "1"^^xsd:nonNegativeInteger
                                       ] ;
                       rdfs:comment "Holds information equivalent to the TCE in the GLEC framework. It includes the shared emission parameters for a particular piece, a group of pieces, a shipment or a customer (not defined at this point in time) on a specific TransportMovement. A TransportMovement (as TOC) can be the base for many TCEs of many customers."@en ;
                       rdfs:label "TransportChainElement"@en .


#################################################################
#    Individuals
#################################################################

###  https://onerecord.iata.org/ns/glecf#LEVEL_1
:LEVEL_1 rdf:type owl:NamedIndividual ,
                  :QualityLevel .


###  https://onerecord.iata.org/ns/glecf#LEVEL_2
:LEVEL_2 rdf:type owl:NamedIndividual ,
                  :QualityLevel .


###  https://onerecord.iata.org/ns/glecf#LEVEL_3
:LEVEL_3 rdf:type owl:NamedIndividual ,
                  :QualityLevel .


###  https://onerecord.iata.org/ns/glecf#LEVEL_4
:LEVEL_4 rdf:type owl:NamedIndividual ,
                  :QualityLevel .


###  Generated by the OWL API (version 4.5.9.2019-02-01T07:24:44Z) https://github.com/owlcs/owlapi
